loads of comments in the proof of Higman's lemma

theories/embeddings/utree_embed.v
@@ -32,9 +32,9 @@ Section utree_embed.
 
   Implicit Types (R : rel₂ X) (T : rel₂ Y).
 
-  Inductive sub_utree : rel₂ (utree X Y) :=
-    | sub_utree_refl t : t ≤ut t
-    | sub_utree_subt s y t : s ≤ut t → s ≤ut ⟨y|t⟩₁
+  Inductive sub_utree s : rel₁ (utree X Y) :=
+    | sub_utree_refl : s ≤ut s
+    | sub_utree_subt y t : s ≤ut t → s ≤ut ⟨y|t⟩₁
   where "s ≤ut t" := (sub_utree s t).
 
   Hint Constructors sub_utree : core.
@@ -57,6 +57,8 @@ Section utree_embed.
     | utree_embed_root y₁ t₁ y₂ t₂ : T y₁ y₂ → t₁ ≤ₑ t₂ → ⟨y₁|t₁⟩₁ ≤ₑ ⟨y₂|t₂⟩₁
   where "s ≤ₑ t" := (@utree_embed _ _ s t).
 
+  Hint Constructors utree_embed : core.
+
   Fact utree_embed_inv_right R T s t :
           utree_embed R T s t
         → match t with
@@ -69,23 +71,121 @@ Section utree_embed.
     right; eauto.
   Qed.
 
+  Fact utree_embed_inv_0_ R T x₁ t :
+         utree_embed R T ⟨x₁⟩₀ t
+       → match t with
+         | ⟨x₂⟩₀    => R x₁ x₂
+         | ⟨y₂|t₂⟩₁ => utree_embed R T ⟨x₁⟩₀ t₂
+         end.
+  Proof.
+    intros H%utree_embed_inv_right; destruct t as [ x1 | y2 t2 ].
+    + destruct H as (? & [=] & ?); now subst.
+    + destruct H as [ | (? & ? & ? & _) ]; now auto.
+  Qed.
+
+  Fact utree_embed_inv_1_ R T y₁ t₁ t :
+         utree_embed R T ⟨y₁|t₁⟩₁ t
+       → match t with
+         | ⟨x₂⟩₀    => False
+         | ⟨y₂|t₂⟩₁ => utree_embed R T ⟨y₁|t₁⟩₁ t₂ ∨ T y₁ y₂ ∧ utree_embed R T t₁ t₂
+         end.
+  Proof.
+    intros H%utree_embed_inv_right; destruct t as [ x1 | y2 t2 ].
+    + now destruct H as (? & ? & _).
+    + destruct H as [ | (? & ? & [=] & []) ]; subst; eauto.
+  Qed.
+
+  Fact utree_embed_inv_1_ex R T y₁ t₁ t :
+         utree_embed R T ⟨y₁|t₁⟩₁ t
+       → ∃ y₂ t₂, utree_embed R T ⟨y₁|t₁⟩₁ t₂ ∨ T y₁ y₂ ∧ utree_embed R T t₁ t₂.
+  Proof.
+    destruct t as [ | y2 t2 ]; intros H%utree_embed_inv_right.
+    + now destruct H as (? & ? & _).
+    + exists y2, t2.
+      destruct H as [ | (? & ? & [=] & []) ]; subst; eauto.
+  Qed.
+
+  Fact utree_embed_inv_10 R T y₁ t₁ x₂ :
+         utree_embed R T ⟨y₁|t₁⟩₁ ⟨x₂⟩₀ → False.
+  Proof. now intros (? & ? & _)%utree_embed_inv_right. Qed.
+
+  Fact utree_embed_inv_11 R T y₁ t₁ y₂ t₂ :
+         utree_embed R T ⟨y₁|t₁⟩₁ ⟨y₂|t₂⟩₁
+       → utree_embed R T ⟨y₁|t₁⟩₁ t₂
+       ∨ T y₁ y₂ ∧ utree_embed R T t₁ t₂.
+  Proof. intros [ | (? & ? & [=] & []) ]%utree_embed_inv_right; subst; eauto. Qed.
+
   Fact utree_sub_embed R T r s t : r ≤ut s → utree_embed R T s t → utree_embed R T r t.
   Proof.
-    induction 1 as [ | r y s H IH ] in t |- *; auto.
+    induction 1 as [ | y s H IH ] in t |- *; auto.
     induction t as  [ x | y' t IHt ].
-    + now intros (? & ? & _)%utree_embed_inv_right.
-    + intros [ ? | (? & ? & [=] & ? & ?) ]%utree_embed_inv_right.
+    + now intros ?%utree_embed_inv_10.
+    + intros [ ? | [] ]%utree_embed_inv_11.
       * constructor 2; eauto.
       * subst; constructor 2; eauto.
   Qed.
 
-  Fact utree_embed_trans R T x s t : utree_embed R T ⟨x|s⟩₁ t → utree_embed R T s t.
-  Proof. apply utree_sub_embed; eauto. Qed.
+  Fact utree_embed_sub R T r s t : utree_embed R T r s → s ≤ut t → utree_embed R T r t.
+  Proof. induction 2; eauto. Qed.
+
+  (** Notice that utree_embed is transtive if R and T are transitive *)
+
+  Fact utree_embed_leaf_iff R T x₁ x₂ : utree_embed R T ⟨x₁⟩₀ ⟨x₂⟩₀ ↔ R x₁ x₂.
+  Proof. split; auto; intros (? & [=] & ?)%utree_embed_inv_right; now subst. Qed.
+  
+  Fact utree_embed_node_iff R T x (_ : R x x) y₁ y₂ : utree_embed R T ⟨y₁|⟨x⟩₀⟩₁ ⟨y₂|⟨x⟩₀⟩₁ ↔ T y₁ y₂.
+  Proof.
+    split; eauto.
+    now intros [ []%utree_embed_inv_10 | [] ]%utree_embed_inv_11.
+  Qed.
+
+  Section utree_embed_trans.
+
+    Variables (R : rel₂ X) (Rtrans : ∀ x₁ x₂ x₃, R x₁ x₂ → R x₂ x₃ → R x₁ x₃)
+              (T : rel₂ Y) (Ttrans : ∀ y₁ y₂ y₃, T y₁ y₂ → T y₂ y₃ → T y₁ y₃).
+
+    Lemma utree_embed_trans r s t : utree_embed R T r s → utree_embed R T s t → utree_embed R T r t.
+    Proof.
+      intros H; revert H t.
+      induction 1 as [ x1 x2 H1 | r y1 s H1 IH1 | y1 r y2 s H1 H2 IH2 ]; intros t.
+      + induction t; intros H%utree_embed_inv_0_; eauto.
+      + induction t; intros H%utree_embed_inv_1_; [ easy | destruct H as [ | [] ] ]; eauto.
+      + induction t; intros H%utree_embed_inv_1_; [ easy | destruct H as [ | [] ] ]; eauto.
+    Qed.
+
+  End utree_embed_trans.
+
+  Section utree_embed_trans_inv.
+
+     Variables (R : rel₂ X) (T : rel₂ Y) (Hute : ∀ r s t, utree_embed R T r s → utree_embed R T s t → utree_embed R T r t).
+
+     Fact utree_embed_trans_0 x₁ x₂ x₃ : R x₁ x₂ → R x₂ x₃ → R x₁ x₃.
+     Proof.
+       intros H1%(utree_embed_leaf_iff R T) H2%(utree_embed_leaf_iff R T).
+       apply (utree_embed_leaf_iff R T); eauto.
+     Qed.
+
+     (** The hypothesis below could be relaxed with (t : utree X Y) (utree_embed R T t t) but that
+         would require more work, in particular to generalize utree_embed_node_iff by replacing 
+         ⟨x⟩₀ with t *)
+     Variables (x : X) (Hx : R x x).
+
+     Fact utree_embed_trans_1 y₁ y₂ y₃ : T y₁ y₂ → T y₂ y₃ → T y₁ y₃.
+     Proof.
+       intros ?%(utree_embed_node_iff R T _ Hx) ?%(utree_embed_node_iff R T _ Hx).
+       apply (utree_embed_node_iff R T _ Hx); eauto.
+     Qed.
+
+     (* Notice that if X is not inhabited then utree X _ is neither (because trees
+        must have leaves) and hence utree_embed R T is transitive (by lack of trees), 
+        regardedless of T *) 
+
+  End utree_embed_trans_inv.
 
 End utree_embed.
 
 #[global] Hint Constructors sub_utree utree_embed : utree_db.
-#[global] Hint Resolve sub_utree_trans : utree_db.
+#[global] Hint Resolve sub_utree_trans utree_sub_embed utree_embed_sub: utree_db.
 
 Module utree_embeddings_notations.
 
